code/ecdsap256/Hacl.Impl.ScalarMultiplication.WNAF.fst
@@ -16,10 +16,32 @@ open Lib.IntTypes.Intrinsics
 open Hacl.Impl.P256.Q.PrimitivesMasking
 
 
+(* Originally lives in P256.Core *)
+(* this piece of code is taken from Hacl.Curve25519 *)
+(* changed Endian for Scalar Bit access *)
+
+inline_for_extraction
+val scalar_bit:
+    s:lbuffer_t MUT uint8 (size 32)
+  -> n:size_t{v n < 256}
+  -> Stack uint64
+    (requires fun h0 -> live h0 s)
+    (ensures  fun h0 r h1 -> h0 == h1 /\  v r <= 1)
+
+let scalar_bit s n =
+  let h0 = ST.get () in
+  mod_mask_lemma ((Lib.Sequence.index (as_seq h0 s) (31 - v n / 8)) >>. (n %. 8ul)) 1ul;
+  assert_norm (1 = pow2 1 - 1);
+  assert (v (mod_mask #U8 #SEC 1ul) == v (u8 1)); 
+  to_u64 ((s.(n /. 8ul) >>. (n %. 8ul)) &. u8 1)
+
+
+
+inline_for_extraction noextract
 let dradix_wnaf = (u64 64)
-
+inline_for_extraction noextract
 let dradix = (u64 32)
-
+inline_for_extraction noextract
 let radix = (u64 5)
 
 inline_for_extraction noextract
@@ -31,9 +53,11 @@ val scalar_rwnaf : out: lbuffer uint64 (size 104) -> scalar: lbuffer uint8 (size
 
 let scalar_rwnaf out scalar = 
   push_frame();
+
+  let in0 = index scalar (size 0) in 
+  let windowStartValue =  (logor (u64 1) (logand (to_u64 in0) (dradix_wnaf -! (u64 1))))  in 
   
- let window = create (size 1) (logor (u64 1) (logand (to_u64 (index scalar (size 0))) (dradix_wnaf -! (u64 1))))  in 
- let d = create (size 1) (u64 0) in 
+ let window = create (size 1) windowStartValue in 
 
  let r = create (size 1) (u64 0) in 
  let r1 = create (size 1) (u64 0) in 
@@ -45,26 +69,36 @@ let scalar_rwnaf out scalar =
     (fun i ->
 
       let h0 = ST.get() in 
-      assume (live h0 window);
-      let wAsVariable : uint64 = index window (size 0) in 
+
+      let wVar : uint64 = index window (size 0) in 
       
-      let w = logand wAsVariable  (dradix_wnaf -! (u64 1)) in 
-	let dToUpload = logand wAsVariable (dradix_wnaf -! (u64 1)) -! dradix in 
-      upd d (size 0) dToUpload;
+      let w = logand wVar  (dradix_wnaf -! (u64 1)) in 
+      
+      let d = logand wVar (dradix_wnaf -! (u64 1)) -! dradix in 
+
       let c = sub_borrow_u64 (u64 0) w dradix r in 
       let c1 = sub_borrow_u64 (u64 0) (u64 0) (index r (size 0)) r1 in 
+      
       let cAsFlag = (u64 0xffffffff) +! c in 
       let r3 = cmovznz2 (index r (size 0)) (index r1 (size 0)) cAsFlag in 
+      
       upd out (size 2 *! i) r3;
       upd out (size 2 *! i +! 1) c;
 
 
-      let wStart = wAsVariable -! (index d (size 0)) in 
-      let windowTemp = shift_right wStart radix in  
-      () 
+      let wStart = shift_right (wVar -! d) radix in 
+      let w0 = wStart +! (shift_left (scalar_bit scalar ((size 1 +! i) *! radix +! (size 1))) (size 1)) in 
+      let w0 = w0 +! (shift_left (scalar_bit scalar ((size 1 +! i) *! radix +! (size 2))) (size 2)) in 
+      let w0 = w0 +! (shift_left (scalar_bit scalar ((size 1 +! i) *! radix +! (size 3))) (size 3)) in 
+      let w0 = w0 +! (shift_left (scalar_bit scalar ((size 1 +! i) *! radix +! (size 4))) (size 4)) in 
+      let w0 = w0 +! (shift_left (scalar_bit scalar ((size 1 +! i) *! radix +! (size 5))) (size 5)) in
+
+      upd window (size 0) w0
 
 
     );
+
+    upd out (size 102) (index window (size 0));
 
 pop_frame()
   
